backend/LTL.v
@@ -100,12 +100,11 @@ Definition call_regs (caller: locset) : locset :=
   match caller with
   | (caller_rf, caller_stack) =>
     (caller_rf,
-     fun l: loc =>
-       match l with
-       | R r => encode_val (Locmap.chunk_of_loc l) Vundef
-       | S Local ofs ty => encode_val (Locmap.chunk_of_loc l) Vundef
-       | S Incoming ofs ty => caller_stack (S Outgoing ofs ty)
-       | S Outgoing ofs ty => encode_val (Locmap.chunk_of_loc l) Vundef
+     fun s: slot =>
+       match s with
+       | Local => ZMap.init Undef
+       | Incoming => caller_stack Outgoing
+       | Outgoing => ZMap.init Undef
        end)
   end.
 
@@ -136,10 +135,10 @@ Definition return_regs (caller callee: locset) : locset :=
   match caller, callee with
   | (caller_rf, caller_stack), (callee_rf, _) =>
     (Regfile.override destroyed_at_call callee_rf caller_rf,
-     fun l =>
-     match l with
-     | S Outgoing ofs q => encode_val (chunk_of_quantity q) Vundef
-     | l => caller_stack l
+     fun s: slot =>
+     match s with
+     | Outgoing => ZMap.init Undef
+     | s => caller_stack s
      end)
   end.
 
@@ -159,10 +158,10 @@ Definition undef_caller_save_regs (ls: locset) : locset :=
   match ls with
   | (rf, stack) =>
     (Regfile.undef_regs destroyed_at_call rf,
-     fun l =>
-     match l with
-     | S Outgoing ofs q => encode_val (chunk_of_quantity q) Vundef
-     | l => stack l
+     fun s: slot =>
+     match s with
+     | Outgoing => ZMap.init Undef
+     | s => stack s
      end)
   end.
 
@@ -372,11 +371,9 @@ Lemma call_regs_correct:
   forall (l: loc) (caller: locset),
   (call_regs caller) @ l = call_regs_spec (Locmap.read caller) l.
 Proof.
-  intros. destruct l, caller.
+  intros. destruct l, caller as [caller_rf caller_stack].
   - reflexivity.
-  - unfold Locmap.get, call_regs, call_regs_spec.
-    destruct sl; try (rewrite decode_encode_undef; auto).
-    unfold Locmap.chunk_of_loc; reflexivity.
+  - simpl. unfold Stack.get. destruct sl; auto using FragBlock.gi.
 Qed.
 
 Local Opaque all_mregs.
@@ -408,7 +405,7 @@ Proof.
       rewrite (in_destroyed_at_call r); auto.
     + rewrite Regfile.override_notin; auto.
       rewrite (notin_destroyed_at_call r); auto.
-  - destruct sl; auto. apply decode_encode_undef.
+  - simpl. unfold Stack.get. destruct sl; auto using FragBlock.gi.
 Qed.
 
 Lemma undef_caller_save_regs_correct:
@@ -422,7 +419,7 @@ Proof.
       rewrite (in_destroyed_at_call r); auto.
     + rewrite Regfile.undef_regs_notin; auto.
       rewrite (notin_destroyed_at_call r); auto.
-  - destruct sl; auto. apply decode_encode_undef.
+  - simpl. unfold Stack.get. destruct sl; auto using FragBlock.gi.
 Qed.
 
 Lemma LTL_undef_regs_Regfile_undef_regs:
